\begin{figure}
\textbf{Translation of Implict Types}\\
\begin{align*}
\typofityp{\iota} &= \iota?\\
\typofityp{\arrow{\hat{A}}{\hat{B}}} &= (\arrow{\typofityp{\hat{A}}}{\typofityp{\hat{B}}})?\\
\end{align*}
\textbf{Elvis Operator Syntactic Sugar}\\
\begin{align*}
\elvis{M}{p} &= \case{M}{\blame{p}}{x}{x}
\end{align*}
\textbf{Translation of Implict Terms}\\
\begin{align*}
\trmofitrm{\hat{x}} &= x\\
\trmofitrm{\hat{\code{null}}} &= \code{null}\\
\trmofitrm{\hat{c}} &= \lift{c}\\
\trmofitrm{\binop{\hat{N}}{\hat{M}}} &= \lift{\binop{\elvisP{\trmofitrm{\hat{N}}}{\blop}}{\elvisP{\trmofitrm{\hat{M}}}{\blop}}} \\
\trmofitrm{\abs{x}{\hat{A}}{\hat{N}}} &= \lift{\abs{x}{\typofityp{\hat{A}}}{\trmofitrm{\hat{N}}}} \\
\trmofitrm{\app{\hat{N}}{\hat{M}}} &= \app{\elvisP{\trmofitrm{\hat{N}}}{\blderef}}{\trmofitrm{\hat{M}}} \\
\trmofitrm{\etrm{M}} &= \trmofetrm{M}\\
\end{align*}
\textbf{Translation of Explicit Terms}\\
\begin{align*}
\trmofetrm{x} &= x\\
\trmofetrm{c} &= c\\
\trmofetrm{\binop{N}{M}} &= \binop{\trmofetrm{N}}{\trmofetrm{M}}\\
\trmofetrm{\code{null}} &= \code{null}\\
\trmofetrm{\lift{N}} &= \lift{\trmofetrm{N}}\\
\trmofetrm{\case{N}{M}{x}{L}} &= \case{\trmofetrm{N}}{\trmofetrm{M}}{x}{\trmofetrm{L}}\\
\trmofetrm{\abs{x}{A}{N}} &= \abs{x}{A}{\trmofetrm{N}}\\
\trmofetrm{\app{N}{M}} &= \app{\trmofetrm{N}}{\trmofetrm{M}}\\
\trmofetrm{\cast{M}{A}{p}{B}} &= \cast{\trmofetrm{M}}{A}{p}{B}\\
\trmofetrm{\blame{p}} &= \blame{p}\\
\trmofetrm{\itrm{\hat{M}}} &= \trmofitrm{\hat{M}} \\
\end{align*}
  \caption{Translation of null blame calculus for sublanguages with explicit and implicit nulls into the base null blame calculus}\label{fig:impsyntax}
\end{figure}
